src/computational_monads/simulation_semantics/constructions/logging/caching_oracle.lean
@@ -18,24 +18,121 @@ def caching_oracle (spec : oracle_spec) [spec.computable] :
 namespace caching_oracle
 
 variables (oa : oracle_comp spec α) (i : spec.ι) (t : spec.domain i) (u : spec.range i)
-  (log : query_log spec)
+  (log : query_log spec) --naming → cache
 
-@[simp] lemma apply_eq : (caching_oracle spec).o i (t, log) = option.rec_on (log.lookup i t)
+@[simp] lemma apply_eq : (caching_oracle spec) i (t, log) = option.rec_on (log.lookup i t)
   (query i t >>= λ u, return (u, log.log_query i t u)) (λ u, return (u, log)) :=
-begin
-  simp only [caching_oracle],
-  induction log.lookup i t; refl,
-end
+by {simp only [caching_oracle, sim_oracle.has_coe_to_fun_def], induction log.lookup i t; refl }
+
+lemma apply_eq_of_lookup_eq_none (hlog : log.lookup i t = none) :
+  (caching_oracle spec) i (t, log) = (query i t >>= λ u, return (u, log.log_query i t u)) :=
+by rw [apply_eq, hlog]
+
+lemma apply_eq_of_lookup_eq_some (u : spec.range i) (hlog : log.lookup i t = some u) :
+  (caching_oracle spec) i (t, log) = return (u, log) :=
+by rw [apply_eq, hlog]
 
 lemma apply_eq_of_not_queried (hlog : log.not_queried i t) :
-  (caching_oracle spec).o i (t, log) = (query i t >>= λ u, return (u, log.log_query i t u)) :=
+  (caching_oracle spec) i (t, log) = (query i t >>= λ u, return (u, log.log_query i t u)) :=
+by rw [apply_eq, (query_log.lookup_eq_none_iff_not_queried _ _ _).2 hlog]
+
+section support
+
+@[simp] lemma support_apply : ((caching_oracle spec) i (t, log)).support = if log.not_queried i t
+  then {x | x.2 = log.log_query i t x.1} else {x | some x.1 = log.lookup i t ∧ x.2 = log} :=
+begin
+  split_ifs with hlog; ext x,
+  { rw [apply_eq_of_not_queried i t log hlog, support_bind_return, support_query,
+      set.top_eq_univ, set.image_univ, set.mem_range, set.mem_set_of_eq],
+    refine ⟨λ h, _, λ h, _⟩,
+    { obtain ⟨u, rfl⟩ := h,
+      refl },
+    { exact ⟨x.1, h ▸ (prod.eq_iff_fst_eq_snd_eq.2 ⟨rfl, rfl⟩)⟩ } },
+  { obtain ⟨u, hu⟩ := log.exists_eq_lookup_of_not_not_queried i t hlog,
+    simp only [apply_eq_of_lookup_eq_some _ _ _ u hu.symm, ← hu, support_return,
+      prod.eq_iff_fst_eq_snd_eq, set.mem_singleton_iff, set.mem_set_of_eq] }
+end
+
+lemma support_apply_of_not_queried (hlog : log.not_queried i t) :
+  ((caching_oracle spec) i (t, log)).support = {x | x.2 = log.log_query i t x.1} :=
+by rw [support_apply, if_pos hlog]
+
+lemma support_apply_of_not_not_queried (hlog : ¬ log.not_queried i t) :
+  ((caching_oracle spec) i (t, log)).support = {x | some x.1 = log.lookup i t ∧ x.2 = log} :=
+by rw [support_apply, if_neg hlog]
+
+/-- If the initial cache has `nodup` for some oracle, then so does the final cache. -/
+lemma nodup_simulate (hlog : (log i).nodup) (x : α × query_log spec)
+  (hx : x ∈ (simulate (caching_oracle spec) oa log).support) : (x.2 i).nodup :=
+begin
+  induction oa using oracle_comp.induction_on with α a α β oa ob hoa hob j t,
+  { rw [simulate_return, support_return, set.mem_singleton_iff] at hx,
+    refine hx.symm ▸ hlog },
+  {
+    sorry,
+  },
+  { by_cases h : log.not_queried j t,
+    { rw [simulate_query, support_apply, if_pos h, set.mem_set_of_eq] at hx,
+      rw [hx, log.nodup_log_query_iff j t x.1 i hlog],
+      refine or.inr ((log.not_queried_iff_not_mem _ _).1 h _) },
+    { rw [simulate_query, support_apply, if_neg h, set.mem_set_of_eq] at hx,
+      exact hx.2.symm ▸ hlog } }
+end
+
+/-- If a value is already cached in the initial state, it has the same cache value after. -/
+lemma lookup_simulate_eq_some_of_lookup_eq_some (x : α × query_log spec)
+  (hx : x ∈ (simulate (caching_oracle spec) oa log).support)
+  (hlog : log.lookup i t = some u) : x.2.lookup i t = some u :=
 begin
   sorry
 end
 
-section support
+/-- If a value isn't cached after simulation, it wasn't cached in the initial state. -/
+lemma lookup_eq_none_of_lookup_simulate_eq_none (x : α × query_log spec)
+  (hx : x ∈ (simulate (caching_oracle spec) oa log).support)
+  (hx' : x.2.lookup i t = none) : log.lookup i t = none :=
+begin
+  sorry
+end
 
+/-- The length of the final cache is at least as long as the initial cache -/
+lemma len_cache_le_len_cache_simulate (x : α × query_log spec)
+  (hx : x ∈ (simulate (caching_oracle spec) oa log).support) :
+  (log i).length ≤ (x.2 i).length :=
+begin
+  sorry
+end
 
+/-- For any query fresh to the initial cache, if there is some output such that query has a cached
+value, then there are also outputs with any other possible cached value.  -/
+lemma exists_log_lookup_eq_some (hlog : log.not_queried i t)
+  (x : α × query_log spec) (hx : x ∈ (simulate (caching_oracle spec) oa log).support)
+  (h : x.2.lookup i t = some u) (u' : spec.range i) :
+  ∃ (y : α × query_log spec) (hy : y ∈ (simulate (caching_oracle spec) oa log).support),
+    y.2.lookup i t = some u' :=
+begin
+  sorry
+end
+
+-- TODO: generalize. Should also work for log→seed probably ?
+/-- Re-running a computation with an old cache doesn't change the possible outputs,
+assuming the old cache was generated by an honest simulation. -/
+theorem support_simulate_bind_simulate' (oa : oracle_comp spec α) :
+  (simulate (caching_oracle spec) oa log >>=
+    λ x, simulate (caching_oracle spec) oa x.2).support =
+      (simulate (caching_oracle spec) oa log).support :=
+begin
+  induction oa using oracle_comp.induction_on with α a α β oa ob hoa hob i t,
+  {
+    simp only [simulate_return, support_bind_return, support_return, set.image_singleton],
+  },
+  {
+    sorry,
+  },
+  {
+    sorry,
+  }
+end
 
 end support
 
